Cpc/Proofs/Rules/Pairwise_cong.lean
@@ -28,14 +28,11 @@ by
       cases args with
       | nil =>
           have hCmdTransArgs :
-              cArgListCongOk (CArgList.cons a1 CArgList.nil) := by
+              cArgListTranslationOk (CArgList.cons a1 CArgList.nil) := by
             simpa [cmdTranslationOk] using hCmdTrans
-          have hAOk : eoCongArgOk a1 := by
-            simpa [cArgListCongOk] using hCmdTransArgs.1
           have hATrans : RuleProofs.eo_has_smt_translation a1 := by
-            simpa [eoCongArgOk, eoHasSmtTranslation,
-              RuleProofs.eo_has_smt_translation] using hAOk.1
-          have hAQuantBindersWf : TermQuantifierBindersWf a1 := hAOk.2
+            simpa [cArgListTranslationOk, eoHasSmtTranslation,
+              RuleProofs.eo_has_smt_translation] using hCmdTransArgs.1
           have hProgPairwiseCong :
               __eo_prog_pairwise_cong a1
                   (Proof.pf (__eo_mk_premise_list (Term.UOp UserOp.and) premises s)) ≠
@@ -133,7 +130,6 @@ by
                       N hN f xs (premiseTermList s premises)
                       hATrans
                       hXsTrans
-                      hAQuantBindersWf
                       hEvidence
                       hProgPairwiseCongListBool
                       hProgPairwiseCongListNN
